mem/MemOpen.v
@@ -23,17 +23,81 @@ Set Implicit Arguments.
 
 Let _memRA: URA.t := (block ==> Z ==> (Excl.t val))%ra.
 
+
+Section AUX.
+  Context `{Σ: GRA.t}.
+  Definition mk_ksimple {X: Type} (PQ: X -> ((Any.t -> ord -> Σ -> Prop) * (Any.t -> Σ -> Prop))):
+    ftspec unit unit := @mk_ftspec _ _ _ X (fun x _ a o => (fst ∘ PQ) x a o) (fun x _ a => (snd ∘ PQ) x a)
+  .
+End AUX.
+
+
+
+Section PROOF.
+  Context `{@GRA.inG memRA Σ}.
+
+  Definition alloc_spec: ftspec unit unit :=
+    (mk_ksimple (fun sz => (
+                     (fun varg o => ⌜varg = [Vint (Z.of_nat sz)]↑ /\ o = ord_pure 0⌝),
+                     (fun vret => Exists b, ⌜vret = (Vptr b 0)↑⌝ **
+                                            Own(GRA.embed ((b, 0%Z) |-> (List.repeat (Vint 0) sz))))
+    ))).
+
+  Definition free_spec: ftspec unit unit :=
+    (mk_ksimple (fun '(b, ofs) => (
+                     (fun varg o => Exists v, ⌜varg = ([Vptr b ofs])↑⌝ **
+                                              Own(GRA.embed ((b, ofs) |-> [v])) **
+                                              ⌜o = ord_pure 0⌝),
+                     top2
+    ))).
+
+  Definition load_spec: ftspec unit unit :=
+    (mk_ksimple (fun '(b, ofs, v) => (
+                     (fun varg o => ⌜varg = ([Vptr b ofs])↑⌝ **
+                                    Own(GRA.embed ((b, ofs) |-> [v])) **
+                                    ⌜o = ord_pure 0⌝),
+                     (fun vret => Own(GRA.embed ((b, ofs) |-> [v])) ** ⌜vret = v↑⌝)
+    ))).
+
+  Definition store_spec: ftspec unit unit :=
+    (mk_ksimple
+       (fun '(b, ofs, v_new) => (
+            (fun varg o => Exists v_old,
+                           ⌜varg = ([Vptr b ofs ; v_new])↑⌝ ** Own(GRA.embed ((b, ofs) |-> [v_old])) ** ⌜o = ord_pure 0⌝),
+            (fun _ => Own(GRA.embed ((b, ofs) |-> [v_new])))
+    ))).
+
+  Definition cmp_spec: ftspec unit unit :=
+    (mk_ksimple
+       (fun '(result, resource) => (
+          (fun varg o =>
+          ((Exists b ofs v, ⌜varg = [Vptr b ofs; Vnullptr]↑⌝ ** ⌜resource = (GRA.embed ((b, ofs) |-> [v]))⌝ ** ⌜result = false⌝) ∨
+           (Exists b ofs v, ⌜varg = [Vnullptr; Vptr b ofs]↑⌝ ** ⌜resource = (GRA.embed ((b, ofs) |-> [v]))⌝ ** ⌜result = false⌝) ∨
+           (Exists b0 ofs0 v0 b1 ofs1 v1, ⌜varg = [Vptr b0 ofs0; Vptr b1 ofs1]↑⌝ **
+                     ⌜resource = (GRA.embed ((b0, ofs0) |-> [v0])) ⋅ (GRA.embed ((b1, ofs1) |-> [v1]))⌝ ** ⌜result = false⌝) ∨
+           (Exists b ofs v, ⌜varg = [Vptr b ofs; Vptr b  ofs]↑⌝ ** ⌜resource = (GRA.embed ((b, ofs) |-> [v]))⌝ ** ⌜result = true⌝) ∨
+           (⌜varg = [Vnullptr; Vnullptr]↑ /\ result = true⌝))
+            ** Own(resource)
+            ** ⌜o = ord_pure 0⌝
+          ),
+          (fun vret => Own(resource) ** ⌜vret = (if result then Vint 1 else Vint 0)↑⌝)
+    ))).
+
+End PROOF.
+
+
+
 Section PROOF.
   Context `{@GRA.inG memRA Σ}.
   Let GURA: URA.t := GRA.to_URA Σ.
   Local Existing Instance GURA.
 
-  Definition MemSbtb: list (gname * fspecbody) :=
-    [("alloc", mk_specbody alloc_spec allocF);
-    ("free",   mk_specbody free_spec freeF);
-    ("load",   mk_specbody load_spec loadF);
-    ("store",  mk_specbody store_spec storeF);
-    ("cmp",    mk_specbody cmp_spec cmpF)
+  Definition MemSbtb: list (gname * kspecbody) :=
+    [("alloc", mk_kspecbody alloc_spec allocF);
+    ("free",   mk_kspecbody free_spec freeF);
+    ("load",   mk_kspecbody load_spec loadF);
+    ("store",  mk_kspecbody store_spec storeF);
+    ("cmp",    mk_kspecbody cmp_spec cmpF)
     ]
   .
 
@@ -45,7 +109,7 @@ Section PROOF.
   |}
   .
 
-  Definition SMemSem: Sk.t -> SModSem.t := (disclose_smodsem ∘ KModSem.to_tgt) ∘ KMemSem.
+  Definition SMemSem: Sk.t -> SModSem.t := (KModSem.to_tgt) ∘ KMemSem.
 
   Definition MemSem: Sk.t -> ModSem.t := (SModSem.to_tgt []) ∘ SMemSem.
 
@@ -55,7 +119,7 @@ Section PROOF.
   |}
   .
 
-  Definition SMem: SMod.t := (disclose_smod ∘ KMod.to_tgt) KMem.
+  Definition SMem: SMod.t := (KMod.to_tgt) KMem.
 
   Definition Mem: Mod.t := SMod.to_tgt (fun _ => []) SMem.
 
